RelationalAlgebra/Equivalence/RAtoFOL/Join.lean
@@ -1,4 +1,5 @@
 import RelationalAlgebra.Equivalence.RAtoFOL.Conversion
+import RelationalAlgebra.FOL.RealizeProperties
 
 variable {dbi q₁ q₂} [struc : FOL.folStruc dbi]
 
@@ -15,36 +16,35 @@ theorem ra_to_fol_evalT.j_def.mp (h : RA.Query.isWellTyped dbi.schema (.j q₁ q
         FirstOrder.Language.BoundedFormula.realize_inf, and_imp]
       intro a_2 a_3 a_4
       have h_dom : t.Dom = ↑(q₁.schema dbi.schema) ∪ ↑(q₂.schema dbi.schema) := by
-        obtain ⟨left, right⟩ := h
-
-        have z₁ := FOL.BoundedQuery.Realize.schema_sub_Dom a_2
-        have z₂ := FOL.BoundedQuery.Realize.schema_sub_Dom a_3
-        simp_all only [FOL.Query.RealizeMin.def, ra_to_fol_query_schema, and_imp,
-          forall_const]
-
-        apply Set.Subset.antisymm a_4 (Set.union_subset z₁ z₂)
+        rw [← ra_to_fol_query_schema h.1, ← ra_to_fol_query_schema h.2, a_4]
 
       have z' : ↑(ra_to_fol_query q₁ dbi.schema).schema ⊆ t.Dom := by simp_all [ra_to_fol_query_schema]
-      use t.restrict (z')
+      use t.restrict z'
       apply And.intro
       . apply ih₁
         . apply And.intro
-          . exact FOL.BoundedQuery.Realize.tuple_restrict2 z' a_2
-          . simp_all
-            simp [PFun.Dom, Part.dom_iff_mem, z', Set.subset_def]
-            intro x a x_1 h_1
-            simp_all only [ra_to_fol_query_schema, Set.subset_union_left]
+          . rw [FOL.BoundedQuery.Realize.enlarge]
+            exact a_2
+            . simp [Set.subset_def, PFun.mem_dom]
+            . rfl
+            . rfl
+          . simp_all only [FOL.Query.RealizeMin.def, and_imp]
+            obtain ⟨left, right⟩ := h
+            rfl
 
       . have z' : ↑(ra_to_fol_query q₂ dbi.schema).schema ⊆ t.Dom := by simp_all [ra_to_fol_query_schema]
-        use t.restrict (z')
+        use t.restrict z'
         apply And.intro
         . apply ih₂
           . apply And.intro
-            . exact FOL.BoundedQuery.Realize.tuple_restrict2 z' a_3
-            . simp_all
-              simp [PFun.Dom, Part.dom_iff_mem, z', Set.subset_def]
-              intro x a x_1 h_1
-              simp_all only [ra_to_fol_query_schema, Set.subset_union_left]
+            . rw [FOL.BoundedQuery.Realize.enlarge]
+              exact a_3
+              . simp [Set.subset_def, PFun.mem_dom]
+              . rfl
+              . rfl
+            . simp_all only [FOL.Query.RealizeMin.def, and_imp, Set.subset_union_left]
+              obtain ⟨left, right⟩ := h
+              rfl
 
         . intro a
           simp only [PFun.mem_restrict, Finset.mem_coe, and_imp, not_and]
@@ -102,52 +102,49 @@ theorem ra_to_fol_evalT.j_def.mpr (h : RA.Query.isWellTyped dbi.schema (.j q₁ 
       simp only [FOL.BoundedQuery.Realize.def, FOL.BoundedQuery.toFormula_and,
         FirstOrder.Language.BoundedFormula.realize_inf]
       apply And.intro
-      · have z := (ih₁ w₁ hw₁)
-        have w_Dom : w₁.Dom = q₁.schema dbi.schema := by
+      · have w_Dom : w₁.Dom = q₁.schema dbi.schema := by
           exact RA.Query.evaluate.validSchema q₁ left w₁ hw₁
         have z' : w₁.Dom ⊆ t.Dom := by simp_all
-        apply FOL.BoundedQuery.Realize.tuple_restrict z.1 z'
-
-        ext a v
-        simp [PFun.mem_restrict]
-        by_cases hc : a ∈ w₁.Dom
-        . simp [PFun.mem_dom] at hc
-          have ⟨y, hy⟩ := hc
-          have z'' := (right_1 a).1 y hy
-          simp_all only [Finset.coe_union, subset_refl, and_self, Set.subset_union_left, true_and]
-        . simp_all only [Finset.coe_union, subset_refl, and_self, Set.subset_union_left, Finset.mem_coe]
-          simp [← Finset.mem_coe, (Set.ext_iff.mp w_Dom.symm) a] at hc
+        simp_all only [Finset.coe_union, and_self, Set.subset_union_left, ← FOL.BoundedQuery.Realize.def]
+        have z := (ih₁ w₁ hw₁)
+        have ⟨h_sub, ht'⟩ : ∃h_sub : w₁.Dom ⊆ t.Dom, t.restrict h_sub = w₁ := by
+          obtain ⟨l, r⟩ := z
+          simp [*]; ext a v; simp [*]
+          simp [Set.ext_iff] at r
           apply Iff.intro
           · intro a_1
-            exact False.elim (hc v a_1)
-          · intro a_1
             obtain ⟨left_1, right_2⟩ := a_1
-            obtain ⟨w, h⟩ := left_1
-            exact False.elim (hc w h)
+            have ⟨v', hv'⟩ := (r a).mpr left_1
+            simp_all [← @Part.eq_some_iff]
+          · intro a_1
+            apply And.intro
+            · simp only [← r a]
+              use v
+            · simp_all only [(right_1 a).1 v a_1]
 
+        exact (FOL.BoundedQuery.Realize.enlarge h_sub ht' (by simp_all [ra_to_fol_query_schema])).mp z.1
 
-      · have z := (ih₂ w₂ hw₂)
-        have w_Dom : w₂.Dom = q₂.schema dbi.schema := by
+      · have w_Dom : w₂.Dom = q₂.schema dbi.schema := by
           exact RA.Query.evaluate.validSchema q₂ right w₂ hw₂
         have z' : w₂.Dom ⊆ t.Dom := by simp_all
-        apply FOL.BoundedQuery.Realize.tuple_restrict z.1 z'
-
-        ext a v
-        simp [PFun.mem_restrict]
-        by_cases hc : a ∈ w₂.Dom
-        . simp [PFun.mem_dom] at hc
-          have ⟨y, hy⟩ := hc
-          have z'' := (right_1 a).2.1 y hy
-          simp_all only [Finset.coe_union, subset_refl, and_self, Set.subset_union_left, true_and]
-        . simp_all only [Finset.coe_union, subset_refl, and_self, Set.subset_union_left, Finset.mem_coe]
-          simp [← Finset.mem_coe, (Set.ext_iff.mp w_Dom.symm) a] at hc
+        simp_all only [Finset.coe_union, and_self, Set.subset_union_left, ← FOL.BoundedQuery.Realize.def]
+        have z := (ih₂ w₂ hw₂)
+        have ⟨h_sub, ht'⟩ : ∃h_sub : w₂.Dom ⊆ t.Dom, t.restrict h_sub = w₂ := by
+          obtain ⟨l, r⟩ := z
+          simp [*]; ext a v; simp [*]
+          simp [Set.ext_iff] at r
           apply Iff.intro
           · intro a_1
-            exact False.elim (hc v a_1)
-          · intro a_1
             obtain ⟨left_1, right_2⟩ := a_1
-            obtain ⟨w, h⟩ := left_1
-            exact False.elim (hc w h)
+            have ⟨v', hv'⟩ := (r a).mpr left_1
+            simp_all [← @Part.eq_some_iff]
+          · intro a_1
+            apply And.intro
+            · simp only [← r a]
+              use v
+            · simp_all only [(right_1 a).2.1 v a_1]
+
+        exact (FOL.BoundedQuery.Realize.enlarge h_sub ht' (by simp_all [ra_to_fol_query_schema])).mp z.1
 
 theorem ra_to_fol_evalT.j_def_eq (h : RA.Query.isWellTyped dbi.schema (.j q₁ q₂))
   (ih₁ : (ra_to_fol_query q₁ dbi.schema).evaluateT dbi = RA.Query.evaluateT dbi q₁)
