RelationalAlgebra/FOL/Evaluate.lean
@@ -1,6 +1,6 @@
 import RelationalAlgebra.FOL.Schema
-import RelationalAlgebra.FOL.RealizeProperties
 import RelationalAlgebra.FOL.RelabelProperties
+import RelationalAlgebra.FOL.Realize
 
 open FOL FirstOrder Language RM Term
 
@@ -18,15 +18,6 @@ theorem realize_query_dom {t : Attribute →. Value} (dbi : DatabaseInstance) {q
   t.Dom = q.schema := by
     ext a
     simp_all [PFun.mem_dom, Finset.mem_coe, Query.evaluateT]
-    obtain ⟨h_realize, h_t_sub_schema⟩ := h_realize
-    apply Iff.intro
-    . intro a_1
-      obtain ⟨w, h_1⟩ := a_1
-      apply h_t_sub_schema
-      exact (PFun.mem_dom t a).mpr (Exists.intro w h_1)
-    . intro a_1
-      have left := BoundedQuery.Realize.schema_sub_Dom h_realize
-      exact Part.dom_iff_mem.mp (left a (h_t_sub_schema (left a a_1)))
 
 def Query.evaluate (dbi : DatabaseInstance) {q : Query dbi.schema} [folStruc dbi] :
   RelationInstance := ⟨q.schema, q.evaluateT dbi, λ _ ht ↦ realize_query_dom dbi ht⟩
