RelationalAlgebra/FOL/RealizeProperties.lean
@@ -5,294 +5,151 @@ open FOL FirstOrder Language RM Term
 namespace FOL
 
 @[simp]
-theorem Term.realizeSome.tuple_restrict {dbi} [folStruc dbi] (t : fol.Term (Attribute ⊕ (Fin n))) {tup tup' : Tuple} {iv : Fin n →. Value} :
-  Term.realizeSome dbi t tup' iv → (h_sub : tup'.Dom ⊆ tup.Dom) → tup' = tup.restrict h_sub → Term.realizeSome dbi t tup iv := by
-    intro h_realize h_sub h_eq
-    simp_all only [«def»]
-    have ⟨t, ht⟩ := Term.cases t
-    subst ht
-    cases t with
-    | inl a => exact h_sub h_realize
-    | inr k => simp_all only [realize_var, Sum.elim_inr]
-
-theorem Term.realizeSome.tuple_restrict2 {dbi} [folStruc dbi] (t : fol.Term (Attribute ⊕ (Fin n))) {tup : Tuple} {iv : Fin n →. Value} :
-  Term.realizeSome dbi t tup iv → (h : ↑t.varFinsetLeft ⊆ tup.Dom) → tup' = tup.restrict h → Term.realizeSome dbi t tup' iv := by
-    intro a h ht
-    simp_all only [«def»]
-    have ⟨t, ht⟩ := Term.cases t
-    subst ht
-    cases t with
-    | inl a => simp [PFun.restrict, Part.restrict]
-    | inr k => simp_all only [realize_var, Sum.elim_inr, varFinsetLeft.eq_2, implies_true]
-
-
-@[simp]
-theorem Relmap.tuple_restrict [folStruc : folStruc dbi] {t t' : Tuple} {tMap : Fin (dbi.schema rn).card → fol.Term (Attribute ⊕ (Fin n))}:
-  folStruc.RelMap (fol.Rel dbi.schema rn) (fun i ↦ realize (Sum.elim t' iv) (tMap i)) →
-  (h : t'.Dom ⊆ t.Dom) → t' = t.restrict h →
-    folStruc.RelMap (fol.Rel dbi.schema rn) (fun i ↦ realize (Sum.elim t iv) (tMap i)) := by
-      intro ht h ht'
-      have z : (ArityToTuple fun i ↦ realize (Sum.elim (t.restrict h) iv) (tMap i)) = (ArityToTuple fun i ↦ realize (Sum.elim t iv) (tMap i)) := by
-        ext a v
-        apply Iff.intro
-        · intro a_1
-          unfold ArityToTuple at *
-          simp_all only [PFun.dom_mk, DatabaseInstance.validSchema_def]
-          split
-          next h_1 =>
-            simp_all only [↓reduceDIte, Part.dom_iff_mem]
-            have ⟨k, hk⟩ := Term.cases (tMap (RelationSchema.index h_1))
-            rw [hk]
-            simp_all only [realize_var]
-            cases k with
-            | inl val => simp_all only [Sum.elim_inl, PFun.mem_restrict, Finset.mem_coe]
-            | inr val_1 => simp_all only [Sum.elim_inr]
-          next h_1 => simp_all only [↓reduceDIte, Part.not_mem_none]
-        · intro a_1
-          unfold ArityToTuple at *
-          simp_all only [PFun.dom_mk, DatabaseInstance.validSchema_def]
-          split
-          next h_1 =>
-            simp_all only [↓reduceDIte]
-            have ⟨k, hk⟩ := Term.cases (tMap (RelationSchema.index h_1))
-            have z := Term.RealizeSome.fromRelMap (RelationSchema.index h_1) ht
-            rw [hk]
-            simp_all only [realize_var]
-            cases k with
-            | inl val =>
-              simp [Part.dom_iff_mem] at z a_1
-              simp [a_1, z]
-            | inr val_1 => simp_all only [Sum.elim_inr]
-          next h_1 => simp_all only [↓reduceDIte, Part.not_mem_none]
-      simp_all only [folStruc_apply_RelMap]
-
-
-@[simp]
-theorem Relmap.tuple_restrict2 [folStruc : folStruc dbi] {t : Tuple} (h : ↑((BoundedQuery.R rn tMap).schema) ⊆ t.Dom) :
-  folStruc.RelMap (fol.Rel dbi.schema rn) (fun i ↦ realize (Sum.elim t iv) (tMap i)) →
-    folStruc.RelMap (fol.Rel dbi.schema rn) (fun i ↦ realize (Sum.elim (PFun.restrict t h) iv) (tMap i)) := by
-      intro ht
-      have z : (ArityToTuple fun i ↦ realize (Sum.elim (t.restrict h) iv) (tMap i)) = (ArityToTuple fun i ↦ realize (Sum.elim t iv) (tMap i)) := by
-        ext a v
-        apply Iff.intro
-        · intro a_1
-          unfold ArityToTuple at *
-          simp_all only [PFun.dom_mk, DatabaseInstance.validSchema_def]
-          split
-          next h_1 =>
-            simp_all only [↓reduceDIte, Part.dom_iff_mem]
-            have ⟨k, hk⟩ := Term.cases (tMap (RelationSchema.index h_1))
-            rw [hk]
-            simp_all only [realize_var]
-            cases k with
-            | inl val => simp_all only [Sum.elim_inl, PFun.mem_restrict, Finset.mem_coe]
-            | inr val_1 => simp_all only [Sum.elim_inr]
-          next h_1 => simp_all only [↓reduceDIte, Part.not_mem_none]
-        · intro a_1
-          simp_all
-          have arityDom := RelationInstance.validSchema.def ht
-          unfold ArityToTuple at *
-          simp_all only [PFun.dom_mk, DatabaseInstance.validSchema_def]
-          split
-          next h_1 =>
-            simp_all only [↓reduceDIte]
-            have ⟨k, hk⟩ := Term.cases (tMap (RelationSchema.index h_1))
-            rw [hk]
-            simp_all only [realize_var]
-            cases k with
-            | inl
-              val =>
-              simp_all only [Sum.elim_inl, PFun.mem_restrict, BoundedQuery.schema.R_def, Set.coe_toFinset,
-                Set.mem_setOf_eq, and_true]
-              simp_all only [BoundedQuery.schema.R_def, Set.coe_toFinset]
-              use RelationSchema.index h_1
-              unfold varFinsetLeft
-              split
-              . simp_all only [var.injEq, Sum.inl.injEq, Finset.mem_singleton]
-              . simp_all only [var.injEq, reduceCtorEq]
-              . simp_all [emptyStructure]
-            | inr val_1 => simp_all only [Sum.elim_inr]
-          next h_1 => simp_all only [↓reduceDIte, Part.not_mem_none]
-      simp_all only [folStruc_apply_RelMap]
-
-
-@[simp]
-theorem BoundedQuery.Realize.tuple_restrict [folStruc dbi] {n : ℕ} {q : BoundedQuery dbi.schema n} {t : Tuple} {iv : Fin n →. Value}
-  : q.Realize dbi t' iv → (h : t'.Dom ⊆ t.Dom) → t' = t.restrict h → q.Realize dbi t iv := by
-    intro a h a_1
+theorem BoundedQuery.Realize.enlarge [folStruc dbi] {tup tup' : Tuple} {iv : Fin n →. Value} {q : BoundedQuery dbi.schema n}
+  (h_sub : tup'.Dom ⊆ tup.Dom)
+  (h_res : tup.restrict h_sub = tup')
+  (h_min : ↑q.schema ⊆ tup'.Dom)
+  : q.Realize dbi tup' iv ↔ q.Realize dbi tup iv := by
     induction q with
-    | R rn tMap =>
-      simp_all only [realizeSome.def, toFormula_rel, BoundedFormula.realize_rel]
-      exact Relmap.tuple_restrict a h rfl
+    | R rn vMap =>
+      simp [Realize]
+      rw [@iff_eq_eq, @Set.mem_def, @Set.mem_def]
+      apply congr rfl
+      ext a v
+      simp [ArityToTuple.def_dite]
+      simp_all only [schema.R_def, Set.coe_toFinset]
+      apply Iff.intro
+      · intro a_1
+        split
+        next h =>
+          simp_all only [↓reduceDIte]
+          have := Term.cases (vMap (RelationSchema.index h))
+          simp_all only [Sum.exists]
+          cases this with
+          | inl h_1 =>
+            obtain ⟨w, h_1⟩ := h_1
+            simp_all only [realize_var, Sum.elim_inl]
+            rw [← h_res] at a_1
+            simp at a_1
+            exact a_1.2
+          | inr h_2 =>
+            obtain ⟨w, h_1⟩ := h_2
+            simp_all only [realize_var, Sum.elim_inr]
+        next h => simp_all only [↓reduceDIte, Part.not_mem_none]
+      · intro a_1
+        split
+        next h =>
+          simp_all only [↓reduceDIte]
+          have := Term.cases (vMap (RelationSchema.index h))
+          simp_all only [Sum.exists]
+          cases this with
+          | inl h_1 =>
+            obtain ⟨w, h_1⟩ := h_1
+            simp_all only [realize_var, Sum.elim_inl]
+            simp [Set.subset_def, PFun.mem_dom] at h_min
+            have ⟨v', h_2⟩ := h_min w (RelationSchema.index h) (by simp_all only [varFinsetLeft.eq_1, Finset.mem_singleton])
+            rw [← h_res] at h_2 ⊢
+            simp at h_2 ⊢
+            simp_all only [and_self]
+          | inr h_2 =>
+            obtain ⟨w, h_1⟩ := h_2
+            simp_all only [realize_var, Sum.elim_inr]
+        next h => simp_all only [↓reduceDIte, Part.not_mem_none]
 
-    | tEq sq t₁ t₂ ih  =>
-      simp_all only [«def», toFormula_tEq, BoundedFormula.realize_inf,
-        true_and, forall_const, implies_true]
-      obtain ⟨left, right⟩ := a
-
-      have hDom₁ := Realize.all_terms left t₁ sorry
-      have hDom₂ := Realize.all_terms left t₂ sorry
-
-      · simp_all [BoundedFormula.Realize]
-        have ⟨t₁, ht₁⟩ := Term.cases t₁
-        have ⟨t₂, ht₂⟩ := Term.cases t₂
-        simp_all [ht₁, ht₂]
-        cases t₁ with
-        | inl att₁ =>
-          simp_all
-          cases t₂ with
-          | inl att₂ =>
-            by_cases hd₁ : (t' att₁).Dom
-            . by_cases hd₂ : (t' att₂).Dom
-              . simp [Part.ext_iff] at right ⊢
-                simp [Part.dom_iff_mem] at hd₁ hd₂
-                intro v
-                apply Iff.intro
-                . intro hv
-                  exact ((right v).mp (And.intro hd₁ hv)).2
-                . intro hv
-                  exact ((right v).mpr (And.intro hd₂ hv)).2
-              . simp_all
-            . simp_all
-          | inr fin₂ =>
-            by_cases (t' att₁).Dom
-            . simp_all
-              rw [← right]
-              ext v
-              simp [PFun.mem_restrict]
-              intro a
-              subst ht₁ ht₂
-              simp_all only
-              exact Part.dom_iff_mem.mp hDom₂
-            . simp_all
-        | inr fin₁ =>
-          cases t₂ with
-          | inl att₂ =>
-            by_cases (t' att₂).Dom
-            . simp_all
-              ext v
-              simp [PFun.mem_restrict]
-              intro a
-              subst ht₁ ht₂
-              simp_all only
-              exact Part.dom_iff_mem.mp hDom₂
-            . simp_all
-          | inr fin₂ =>
-            simp_all
-
-    | ex q ih =>
-      simp [BoundedQuery.Realize.def] at a ⊢
-      have ⟨w, hw⟩ := a
-      use w
-      simp_all only [«def», forall_const]
-
-    | or q₁ q₂ ih₁ ih₂ =>
-      simp [BoundedQuery.Realize.def] at ⊢ ih₁ ih₂ a
-      simp_all only [forall_const]
-      cases a with
-      | inl h_1 => simp_all only [true_or]
-      | inr h_2 => simp_all only [or_true]
-
-    | not q ih => simp_all [BoundedQuery.Realize.def]; sorry
-
-    | _ => simp_all [BoundedQuery.Realize.def]
-
-@[simp]
-theorem BoundedQuery.Realize.tuple_restrict2 [folStruc dbi] {n : ℕ} {q : BoundedQuery dbi.schema n} {t : Tuple} {iv : Fin n →. Value}
-  : (h : ↑q.schema ⊆ t.Dom) → q.Realize dbi t iv → q.Realize dbi (t.restrict h) iv := by
-    intro h h_rel
-    induction q with
-    | R rn tMap =>
-      simp_all [Relmap.tuple_restrict2 h h_rel,BoundedQuery.Realize.def]
-
-
-    | tEq sq t₁ t₂ ih  =>
-      simp only [«def», toFormula_tEq, BoundedFormula.realize_inf,
-        true_and, forall_const, implies_true, BoundedQuery.Realize.def] at h_rel ⊢
-      simp_all
-      obtain ⟨left, right⟩ := h_rel
-
-      have hDom₁ := Realize.all_terms left t₁ sorry
-      have hDom₂ := Realize.all_terms left t₂ sorry
-
+    | tEq q t₁ t₂ =>
+      simp_all [Realize, BoundedFormula.Realize]
       have ⟨t₁, ht₁⟩ := Term.cases t₁
-      subst ht₁
       have ⟨t₂, ht₂⟩ := Term.cases t₂
-      subst ht₂
-
-      simp_all only [«def», realize_var, true_and]
+      subst ht₁ ht₂
+      intro h
+      simp_all
+      obtain ⟨left, right⟩ := h_min
+      obtain ⟨left_1, right⟩ := right
       cases t₁ with
       | inl val =>
         cases t₂ with
-        | inl val_1 =>
-          simp_all only [Sum.elim_inl, hasSafeTerm_mem_schema]
-          ext a : 1
-          simp_all only [Part.dom_iff_mem, BoundedFormula.Realize, realize_var, Sum.elim_inl,
-            schema, PFun.mem_restrict, Finset.mem_coe, true_and]
-          sorry
-        | inr val_2 =>
-          simp_all only [Sum.elim_inl, hasSafeTerm_mem_schema, Sum.elim_inr]
-          simp_all only [BoundedFormula.Realize, realize_var, Sum.elim_inl, Sum.elim_inr]
-          ext a : 1
-          simp_all only [PFun.mem_restrict, schema.tEq_def, Finset.mem_coe, true_and]
-          sorry
+        | inl
+          val_1 =>
+          simp_all only [varFinsetLeft, Finset.coe_singleton, Set.singleton_subset_iff, PFun.mem_dom, Sum.elim_inl]
+          obtain ⟨w, h_1⟩ := left_1
+          obtain ⟨w_1, h_2⟩ := right
+          apply Iff.intro
+          · intro a
+            rw [← h_res] at a h_1 h_2
+            rw [Part.ext_iff] at a
+            ext v
+            simp at *
+            simp [*] at *
+            exact a v
+
+          · intro a
+            rw [← h_res] at h_1 h_2 ⊢
+            ext v
+            simp at *
+            simp_all only
+        | inr
+          val_2 =>
+          simp_all only [varFinsetLeft, Finset.coe_singleton, Set.singleton_subset_iff, PFun.mem_dom,
+            Finset.coe_empty, Set.empty_subset, Sum.elim_inl, Sum.elim_inr]
+          obtain ⟨w, h_1⟩ := left_1
+          apply Iff.intro
+          · intro a
+            rw [← h_res] at a
+            rw [Part.ext_iff] at a
+            ext v
+            simp at *
+            have : (∃ y, y ∈ tup' val) = True := by aesop
+            simp [this] at a
+            exact a v
+          · intro a
+            rw [← h_res] at h_1 ⊢
+            ext v
+            simp at *
+            simp_all only [true_and]
       | inr val_1 =>
         cases t₂ with
-        | inl val =>
-          simp_all only [Sum.elim_inr, Sum.elim_inl, hasSafeTerm_mem_schema]
-          ext a : 1
-          simp_all only [Part.dom_iff_mem, BoundedFormula.Realize, realize_var, Sum.elim_inr,
-            Sum.elim_inl, schema, PFun.mem_restrict, Finset.mem_coe, true_and]
-          sorry
-        | inr val_2 =>
-          simp_all only [Sum.elim_inr]
-          exact right
+        | inl
+          val =>
+          simp_all only [varFinsetLeft, Finset.coe_empty, Set.empty_subset, Finset.coe_singleton,
+            Set.singleton_subset_iff, PFun.mem_dom, Sum.elim_inr, Sum.elim_inl]
+          obtain ⟨w, h_1⟩ := right
+          apply Iff.intro
+          · intro a
+            rw [← h_res] at a
+            rw [Part.ext_iff] at a
+            ext v
+            simp at *
+            have : (∃ y, y ∈ tup' val) = True := by aesop
+            simp [this] at a
+            exact a v
+          · intro a
+            rw [← h_res] at h_1 ⊢
+            ext v
+            simp at *
+            simp_all only [true_and]
+        | inr val_2 => simp_all only [varFinsetLeft, Finset.coe_empty, Set.empty_subset, Sum.elim_inr]
 
-    | and q₁ q₂ ih₁ ih₂ =>
-      simp only [«def», toFormula_and, BoundedFormula.realize_inf,
-        forall_const, implies_true] at h_rel ⊢
-      simp_all
-      obtain ⟨left_1, right_1⟩ := h_rel
-      apply And.intro
-      · have h': ↑q₁.schema ⊆ t.Dom := by simp_all
-        have := ih₁ h' left_1
-        have h'' : ↑q₁.schema ⊆ ↑(q₁.and q₂).schema := by simp
-        exact tuple_restrict (ih₁ h' left_1) h'' rfl
-      · have h': ↑q₂.schema ⊆ t.Dom := by simp_all
-        have := ih₂ h' right_1
-        have h'' : ↑q₂.schema ⊆ ↑(q₁.and q₂).schema := by simp
-        exact tuple_restrict (ih₂ h' right_1) h'' rfl
+    | and => simp_all [Realize]
 
     | ex q ih =>
-      simp only [«def», toFormula_ex, BoundedFormula.realize_ex, Nat.succ_eq_add_one] at h_rel ⊢
-      simp_all only [«def», forall_const]
-      obtain ⟨w, h_1⟩ := h_rel
-      apply Exists.intro
-      · apply @ih
-        simp_all only [schema.ex_def, forall_true_left]
-        apply h_1
+      simp [Realize]
+      simp_all only [schema.ex_def, forall_const]
+      apply Iff.intro
+      · intro ⟨w, h⟩
+        use w
+        apply ih.mp
+        simp [Realize, h]
+      · intro ⟨w, h⟩
+        use w
+        apply ih.mpr
+        simp [Realize, h]
 
     | or q₁ q₂ ih₁ ih₂ =>
-      simp only [«def», toFormula_or, BoundedFormula.realize_sup,
-        schema.or_def] at h_rel ⊢
-      cases h_rel with
-      | inl left_1 =>
-        have h': ↑q₁.schema ⊆ t.Dom := by simp_all
-        have := ih₁ h' left_1
-        have h'' : ↑q₁.schema ⊆ ↑(q₁.and q₂).schema := by simp
-        apply Or.inl
-        exact tuple_restrict (ih₁ h' left_1) h'' rfl
-      | inr right_1 =>
-        have h': ↑q₂.schema ⊆ t.Dom := by simp_all
-        have := ih₂ h' right_1
-        have h'' : ↑q₂.schema ⊆ ↑(q₁.and q₂).schema := by simp
-        apply Or.inr
-        exact tuple_restrict (ih₂ h' right_1) h'' rfl
+      simp [Realize]
+      simp [← Realize.def]
+      simp_all only [schema.or_def, Finset.coe_union, Set.union_subset_iff]
 
     | not q ih =>
-      simp only [«def», toFormula_not, BoundedFormula.realize_not,
-        schema.not_def] at h_rel ⊢
-      simp_all only [«def», forall_const]
-      apply Aesop.BuiltinRules.not_intro
-      intro a
-      sorry
+      simp [Realize]
+      simp [← Realize.def]
+      simp_all only [schema.not_def]
